hint_set merged to core

OrdSet.v
@@ -7,7 +7,7 @@
    increasing list according to the order relation on elemets of ordType (i.e, <b)
    
    Following list operations are defined on sets:
-    
+   remove a l    ==> removes the first occurence of a from l 
    add a l       ==> adds a to the ordered list l (works only for ordered lists)
    inter l s     ==> returns intersection of sets represented by lists l and s
    union l s     ==> returns union of sets represented by lists l and s
@@ -15,6 +15,10 @@
 
    Some useful results:
 
+
+   Lemma remove_IsOrd (a:A)(l: list A): IsOrd l -> IsOrd (remove a l).
+   Lemma remove_nodup (a:A)(l: list A): NoDup l -> NoDup (remove a l).
+   
    Lemma set_add_IsOrd (a:A)(l: list A): IsOrd(l) -> IsOrd(add a l).
    Lemma set_add_nodup (a:A)(l: list A): IsOrd l -> NoDup (add a l).
   
@@ -45,7 +49,71 @@ Section OrderedSet.
   Definition empty: list A:= nil.
   
   Lemma empty_spec : Empty (empty).
-  Proof.  unfold Empty.  auto with hint_list. Qed.
+  Proof.  unfold Empty.  auto. Qed.
+  
+   
+(*------------ list remove operation on ordered list ----------------------------------- *)
+   Fixpoint rmv (a:A)(l: list A): list A:=
+    match l with
+    |nil => nil
+    | a1::l1 => match comp a a1 with
+               |Eq => l1
+               |Lt => a1:: rmv a l1
+               |Gt => a1:: rmv a l1
+               end
+    end. (* This function deletes only the first occurence of 'a' from the list l *)
+  
+  Lemma set_rmv_elim1 (a b:A)(l: list A): In a (rmv b l)-> In a l.
+  Proof. { induction l. simpl. auto.
+         { simpl. destruct (on_comp b a0).
+           { right;auto. }
+           { intro H1. destruct H1. left;auto. right;auto. }
+           { intro H1. destruct H1. left;auto. right;auto. } } } Qed.
+  Lemma set_rmv_elim2 (a b:A)(l: list A): NoDup l -> In a (rmv b l)-> (a<>b).
+  Proof. { induction l. simpl. auto.
+         { simpl. destruct (on_comp b a0).
+           { intros H1 H2. subst b. intro H3. subst a.
+             absurd (In a0 l); eauto. }
+           { intros H1 H2. destruct H2. intro. subst a0; subst a.
+             absurd (b <b b); eauto. eauto. }
+           { intros H1 H2. destruct H2. intro. subst a0; subst a.
+             absurd (b <b b); eauto. eauto. } } } Qed.
+  
+  Lemma set_rmv_intro (a b: A)(l:list A): In a l -> a<>b -> In a (rmv b l).
+  Proof. { induction l. simpl.  auto.
+         { simpl. destruct (on_comp b a0).
+           { intros H1 H2. destruct H1. subst a; subst b.
+             absurd (a0=a0); auto. auto. }
+           { intros H1 H2. simpl. destruct H1. left;auto. right;auto. }
+           { intros H1 H2. simpl. destruct H1. left;auto. right;auto. } } } Qed.
+           
+  Hint Resolve set_rmv_elim1 set_rmv_elim2 set_rmv_intro: core.
+  Lemma set_rmv_iff (a b:A)(l: list A): NoDup l -> (In a (rmv b l) <-> (In a l /\ a<>b)).
+  Proof. intro H. split. eauto.
+         intro H0. destruct H0 as [H0 H1]. eauto.  Qed. 
+  
+  Lemma set_rmv_IsOrd (a:A)(l: list A): IsOrd l -> IsOrd (rmv a l).
+  Proof. { induction l. simpl.  constructor.
+         { intro H. simpl. destruct (on_comp a a0).
+           { eauto. }
+           { apply IsOrd_intro. eauto. intros x H1.
+             cut(In x l); eauto.  }
+            { apply IsOrd_intro. eauto. intros x H1.
+              cut(In x l). intros; eapply IsOrd_elim2a; eauto. eauto. } } } Qed.
+
+  
+           
+  
+  Lemma set_rmv_nodup (a:A)(l: list A): NoDup l -> NoDup (rmv a l).
+  Proof.  { induction l. simpl. constructor.
+          { intro H. simpl. destruct (on_comp a a0).
+            { eauto. }
+            { constructor. intro H1. absurd (In a0 l). eauto.
+              eauto. eauto. }
+            { constructor. intro H1. absurd (In a0 l). eauto.
+              eauto. eauto. } } } Qed.
+
+  Hint Resolve set_rmv_IsOrd set_rmv_nodup: core.
 
  
    (* ------------ set_add operation for ordered list -------------- ---------------  *)
@@ -63,56 +131,56 @@ Section OrderedSet.
   Lemma set_add_intro1 (a b: A)(l: list A): In a l -> In a (add b l).
   Proof. { intro H. induction l.  inversion H.
          destruct H.
-         { subst a0. simpl; destruct (on_comp b a); eauto with hint_list. }
-         { simpl; destruct (on_comp b a0); eauto with hint_list. } } Qed.
+         { subst a0. simpl; destruct (on_comp b a); eauto. }
+         { simpl; destruct (on_comp b a0); eauto. } } Qed.
   
-  Lemma set_add_intro2 (a b: A)(l: list A): a=b -> In a (add b l).
+  Lemma set_add_intro2 (a b: A)(l: list A): a= b -> In a (add b l).
   Proof. { intro. subst a. induction l.
          simpl. left;auto. simpl. destruct (on_comp b a).
-         subst b; auto with hint_list. all: auto with hint_list. } Qed.
-  Lemma set_add_intro (a b: A)(l: list A): (a=b \/ In a l) -> In a (add b l).
+         subst b; auto. all: auto. } Qed.
+  Lemma set_add_intro (a b: A)(l: list A): (a= b \/ In a l) -> In a (add b l).
   Proof. intro H. destruct H.  eapply set_add_intro2;auto.  eapply set_add_intro1;auto. Qed.
   Lemma set_add_intro3 (a:A)(l: list A): In a (add a l).
-  Proof. { eapply set_add_intro2. auto.  } Qed.
-  Hint Resolve set_add_intro set_add_intro1 set_add_intro2 set_add_intro3: hint_list.
+  Proof. { eapply set_add_intro2;auto.  } Qed.
+  Hint Resolve set_add_intro set_add_intro1 set_add_intro2 set_add_intro3: core.
   
   Lemma set_add_not_empty (a: A)(l:list A): add a l <> (empty).
   Proof. intro H. absurd (In a empty). simpl; auto. rewrite <- H.
-         eauto with hint_list. Qed. 
+         eauto. Qed. 
     
-  Lemma set_add_elim (a b: A)(l: list A): In a (add b l)-> ( a=b \/ In a l).
+  Lemma set_add_elim (a b: A)(l: list A): In a (add b l)-> ( a= b \/ In a l).
   Proof. { induction l.
          simpl. left. symmetry. tauto. intro H.
          simpl in H. destruct (on_comp b a0).
          right;auto. destruct H. left; subst b;auto. right;auto.
-         destruct H. right; subst a0; eauto with hint_list.
-         apply IHl in H. destruct H; eauto with hint_list. } Qed.
+         destruct H. right; subst a0; auto.
+         apply IHl in H. destruct H; auto. } Qed.
   
-  Lemma set_add_elim1 (a b: A)(l: list A): In a (add b l)-> ~ In a l -> a=b.
+  Lemma set_add_elim1 (a b: A)(l: list A): In a (add b l)-> ~ In a l -> a= b.
   Proof. { intros H H0.
-         assert (H1: a=b \/ In a l). eapply set_add_elim;eauto.
+         assert (H1: a= b \/ In a l). apply set_add_elim;auto.
          destruct H1. auto. absurd (In a l);auto. } Qed.
   Lemma  set_add_elim2 (a b: A)(l: list A): In a (add b l)-> a<>b-> In a l.
   Proof. { intros H H0.
-         assert (H1: a=b \/ In a l). eapply set_add_elim;eauto.
-         destruct H1. absurd (a=b); auto. auto. } Qed.
+         assert (H1: a= b \/ In a l). apply set_add_elim;auto.
+         destruct H1. absurd (a= b); auto. auto. } Qed.
   
-  Hint Resolve set_add_elim set_add_elim1 set_add_elim2: hint_list.
-  Lemma set_add_iff (a b:A)(l:list A): In a (add b l) <-> (a=b \/ In a l).
-  Proof. split; auto with hint_list. Qed.
+  Hint Resolve set_add_elim set_add_elim1 set_add_elim2: core.
+  Lemma set_add_iff (a b:A)(l:list A): In a (add b l) <-> (a= b \/ In a l).
+  Proof. split; auto. Qed.
   
   Lemma set_add_IsOrd (a:A)(l: list A): IsOrd(l) -> IsOrd(add a l).
   Proof. { induction l. simpl. constructor.
          { intro H.  simpl. destruct (on_comp a a0).
            auto. constructor;auto.
-           apply IsOrd_intro. eauto with hint_list.
-           intros x H1. assert(H2: x=a \/ In x l). auto with hint_list.
-           destruct H2. subst x;auto. eauto with hint_list. } } Qed.
+           apply IsOrd_intro. eauto.
+           intros x H1. assert(H2: x=a \/ In x l). auto.
+           destruct H2. subst x;auto. eapply IsOrd_elim2a; eauto.  } } Qed.
   
   Lemma set_add_nodup (a:A)(l: list A): IsOrd l -> NoDup (add a l).
-  Proof. intro H. cut (IsOrd (add a l)). auto with hint_list. apply set_add_IsOrd;auto. Qed.
+  Proof. intro H. cut (IsOrd (add a l)). auto. apply set_add_IsOrd;auto. Qed.
 
-  Hint Resolve set_add_IsOrd set_add_nodup : hint_list. 
+  Hint Resolve set_add_IsOrd set_add_nodup : core. 
  
   (* ------------ set_inter operation ----------------------------------------------  *)
   
@@ -129,16 +197,16 @@ Section OrderedSet.
   Proof. { induction x.
          { intro H; inversion H. }
          { intros H H1.
-           assert (H2: a=a0 \/ In a x); auto with hint_list.
+           assert (H2: a=a0 \/ In a x); auto.
            destruct H2.
-           { subst a0. simpl. destruct (mem a y) eqn: H2. auto with hint_list.
+           { subst a0. simpl. destruct (mem a y) eqn: H2. auto.
              absurd (mem a y). switch;auto.  apply /memP;auto. }
-           { simpl. destruct (mem a0 y) eqn: H2; eauto with hint_list. } } } Qed.
+           { simpl. destruct (mem a0 y) eqn: H2; auto. } } } Qed.
   Lemma set_inter_elim1 (a:A)(x y: list A): In a (inter x y)-> In a x.
   Proof. { induction x.
          { simpl. tauto. }
          { simpl. destruct (mem a0 y).
-           { intro H0. assert(H: a= a0 \/ In a (inter x y)); auto with hint_list.
+           { intro H0. assert(H: a= a0 \/ In a (inter x y)); auto.
              destruct H. left;symmetry;auto. right;auto. }
            { intro;right;auto. } } } Qed.
                       
@@ -146,7 +214,7 @@ Section OrderedSet.
   Proof. { induction x.
          { simpl. tauto. }
          { simpl. destruct (mem a0 y) eqn: Hy.
-           { intro H0. assert(H: a=a0 \/ In a (inter x y));auto with hint_list.
+           { intro H0. assert(H: a=a0 \/ In a (inter x y));auto.
              destruct H. subst a; apply /memP;auto. auto. }
            { auto. } } } Qed.
   
@@ -156,25 +224,29 @@ Section OrderedSet.
   Lemma set_inter_IsOrd (x y: list A): IsOrd (inter x y).
   Proof. { induction x.
          { simpl. constructor. }
-         { simpl. destruct (mem a y); eauto with hint_list. } } Qed.
+         { simpl. destruct (mem a y); auto. } } Qed.
   
   Lemma set_inter_nodup (x y:list A): NoDup (inter x y).
   Proof. { induction x.
          { simpl. constructor. }
          { simpl.  assert (H1: IsOrd (inter x y)). apply set_inter_IsOrd.
-           destruct (mem a y); eauto with hint_list. } } Qed.
+           destruct (mem a y); auto. } } Qed.
 
-  Hint Resolve set_inter_intro set_inter_elim1 set_inter_elim2: hint_list.
-  Hint Resolve set_inter_IsOrd set_inter_nodup: hint_list.
+  Hint Resolve set_inter_intro set_inter_elim1 set_inter_elim2: core.
+  Hint Resolve set_inter_IsOrd set_inter_nodup: core.
   
   Lemma set_inter_comm (x y:list A): Equal (inter x y) (inter y x).
-  Proof. split; intro H; cut (In a x); cut (In a y); eauto with hint_list. Qed.
+  Proof.  { split; intros a H.
+         assert (H1: In a x /\ In a y). split;eauto.
+         destruct H1; auto.
+         assert (H1: In a y /\ In a x). split;eauto.
+         destruct H1; auto. }  Qed.
 
-  Hint Resolve set_inter_comm: hint_list.
+  Hint Resolve set_inter_comm: core.
 
   Lemma inter_equal (x y:list A): inter x y = inter y x.
-  Proof.  assert (H1: Equal (inter x y) (inter y x)). auto with hint_list.
-          cut (IsOrd (inter x y)); cut (IsOrd (inter y x)); eauto with hint_list. Qed.
+  Proof.  assert (H1: Equal (inter x y) (inter y x)). auto.
+          cut (IsOrd (inter x y)); cut (IsOrd (inter y x)); eauto. Qed.
   
      
   (* ------------ set_union operation ----------------------------------------------  *)
@@ -187,47 +259,47 @@ Section OrderedSet.
 
   Lemma set_union_intro1 (a:A)(l s: list A): In a l -> In a (union l s).
   Proof. { induction l. simpl. tauto.
-         simpl. intro H; destruct H. subst a. auto with hint_list.
-         auto with hint_list. } Qed.
+         simpl. intro H; destruct H. subst a. auto.
+         auto. } Qed.
   Lemma set_union_intro2 (a:A)(l s: list A): In a s -> In a (union l s).
-  Proof. induction l. simpl. auto. simpl. auto with hint_list. Qed.
+  Proof. induction l. simpl. auto. simpl. auto. Qed.
   
   Lemma set_union_elim (a:A)(l s:list A): In a (union l s) -> (In a l \/ In a s).
   Proof. { induction l. simpl. right;auto.
          simpl. intro H.
-         assert (H1: a=a0 \/ In a (union l s)); auto with hint_list.
+         assert (H1: a=a0 \/ In a (union l s)); auto.
          destruct H1.
          { left. left. symmetry;auto. }
          { assert (H1: In a l \/ In a s);auto. destruct H1. left;right;auto.
            right;auto. } } Qed.
-  Hint Resolve set_union_intro1 set_union_intro2 set_union_elim: hint_list.
+  Hint Resolve set_union_intro1 set_union_intro2 set_union_elim: core.
   
   Lemma set_union_IsOrd (x y: list A): IsOrd y -> IsOrd (union x y).
   Proof. { induction x.
          { simpl. auto.  }
-         { intros H1. simpl.  eauto with hint_list. } } Qed.
+         { intros H1. simpl.  auto. } } Qed.
   Lemma set_union_nodup (x y: list A): IsOrd y -> NoDup (union x y).
   Proof. { induction x.
-         { simpl. auto with hint_list.  }
-         { intros H1. simpl. cut(IsOrd (add a (union x y))).  eauto with hint_list.
-           cut (IsOrd (union x y)). eauto with hint_list. apply set_union_IsOrd;auto. } } Qed.
+         { simpl. auto.  }
+         { intros H1. simpl. cut(IsOrd (add a (union x y))).  auto.
+           cut (IsOrd (union x y)). auto. apply set_union_IsOrd;auto. } } Qed.
   Lemma set_union_comm (x y:list A): Equal (union x y) (union y x).
-  Proof. { split; intro H.
-         assert (H1: In a x \/ In a y); auto with hint_list.
-         destruct H1; auto with hint_list.
-         assert (H1: In a y \/ In a x); auto with hint_list.
-         destruct H1; auto with hint_list. } Qed.
+  Proof. { split; intros a H.
+         assert (H1: In a x \/ In a y); auto.
+         destruct H1; auto.
+         assert (H1: In a y \/ In a x); auto.
+         destruct H1; auto. } Qed.
   
-  Hint Resolve set_union_IsOrd set_union_nodup  : hint_list.
+  Hint Resolve set_union_IsOrd set_union_nodup  : core.
 
   Lemma union_equal (x y:list A): IsOrd x -> IsOrd y -> union x y = union y x.
   Proof. { intros.
          cut (Equal (union x y) (union y x)).
          cut (IsOrd (union x y)). cut (IsOrd (union y x)).
-         eauto with hint_list. all: eauto with hint_list.
+         eauto. all: eauto.
          apply set_union_comm. } Qed.
   
-  Hint Resolve inter_equal union_equal set_union_comm: hint_list.
+  Hint Resolve inter_equal union_equal set_union_comm: core.
 
   
   (* ------------ set_diff operation -----------------------------------------------  *)
@@ -243,59 +315,62 @@ Section OrderedSet.
 
   Lemma set_diff_intro (a: A)(l s: list A): In a l -> ~In a s -> In a (diff l s).
   Proof. { induction l.
-         { simpl. auto. }
+         { simpl; auto. }
          { intros H H1. simpl.
-           assert (H0: a=a0 \/ In a l); auto with hint_list.
+           assert (H0: a=a0 \/ In a l); auto.
            destruct H0.
            destruct (mem a0 s) eqn:H2.
            { absurd ( In a0 s). subst a0;auto. apply /memP;auto. }
-           { subst a0. auto with hint_list. }
-           destruct (mem a0 s) eqn:H2. eauto.
-           cut (In a (diff l s)); auto with hint_list. } } Qed.
+           { subst a0; auto. }
+           destruct (mem a0 s) eqn:H2. auto.
+           cut (In a (diff l s)); auto. } } Qed.
            
   Lemma set_diff_elim1 (a:A)(l s: list A): In a (diff l s) -> In a l.
   Proof. { induction l. simpl; auto.
          { simpl. destruct (mem a0 s) eqn: H0.
            intro; right; auto. intro H1.
-           assert (H2: a= a0 \/ In a (diff l s)); auto with hint_list.
+           assert (H2: a= a0 \/ In a (diff l s)); auto.
            destruct H2. left; symmetry;auto. right;auto. } } Qed.
   Lemma set_diff_elim2 (a:A)(l s: list A): In a (diff l s) -> ~In a s.
   Proof. { induction l. simpl;auto.
          { simpl. destruct (mem a0 s) eqn: H0.
-           auto. intro H1. assert (H2: a= a0 \/ In a (diff l s)). auto with hint_list.
+           auto. intro H1. assert (H2: a= a0 \/ In a (diff l s)); auto.
            destruct H2. subst a. move /memP. switch_in H0. auto. auto. } } Qed.
   Lemma set_diff_empty (a:A)(l: list A): ~ In a (diff l l).
   Proof. intro H. absurd (In a l). eapply set_diff_elim2;eauto.
          eapply set_diff_elim1;eauto. Qed.
 
-  Hint Resolve set_diff_elim1 set_diff_elim2 set_diff_intro set_diff_empty: hint_list.
+  Hint Resolve set_diff_elim1 set_diff_elim2 set_diff_intro set_diff_empty: core.
 
   Lemma set_diff_IsOrd (l s: list A): IsOrd (diff l s).
   Proof. { induction l.
            { simpl. constructor. }
-           { simpl. destruct (mem a s); eauto with hint_list. } } Qed.
+           { simpl. destruct (mem a s); auto. } } Qed.
   
   Lemma set_diff_nodup (l s: list A): NoDup (diff l s).
-  Proof. cut (IsOrd (diff l s)). auto with hint_list. apply set_diff_IsOrd. Qed.
+  Proof. cut (IsOrd (diff l s)). auto. apply set_diff_IsOrd. Qed.
 
-  Hint Resolve set_diff_IsOrd set_diff_nodup: hint_list.
+  Hint Resolve set_diff_IsOrd set_diff_nodup: core.
           
 End OrderedSet.
 
 
-  
 
-Hint Resolve set_add_intro set_add_intro1 set_add_intro2 set_add_intro3: hint_list.
-Hint Resolve set_add_elim set_add_elim1 set_add_elim2: hint_list.
-Hint Resolve set_add_IsOrd set_add_nodup: hint_list.
 
-Hint Resolve set_inter_intro set_inter_elim1 set_inter_elim2 set_inter_comm: hint_list.
-Hint Resolve set_inter_IsOrd set_inter_nodup : hint_list.
+Hint Resolve set_rmv_elim1 set_rmv_elim2 set_rmv_intro: core.
+Hint Resolve set_rmv_IsOrd set_rmv_nodup: core.
 
-Hint Resolve set_union_intro1 set_union_intro2 set_union_elim set_union_comm: hint_list.
-Hint Resolve set_union_IsOrd set_union_nodup  : hint_list.
+Hint Resolve set_add_intro set_add_intro1 set_add_intro2 set_add_intro3: core.
+Hint Resolve set_add_elim set_add_elim1 set_add_elim2: core.
+Hint Resolve set_add_IsOrd set_add_nodup: core.
 
-Hint Resolve inter_equal union_equal: hint_list.
+Hint Resolve set_inter_intro set_inter_elim1 set_inter_elim2 set_inter_comm: core.
+Hint Resolve set_inter_IsOrd set_inter_nodup : core.
 
-Hint Resolve set_diff_elim1 set_diff_elim2 set_diff_intro set_diff_empty: hint_list.
-Hint Resolve set_diff_IsOrd set_diff_nodup: hint_list.
+Hint Resolve set_union_intro1 set_union_intro2 set_union_elim set_union_comm: core.
+Hint Resolve set_union_IsOrd set_union_nodup  : core.
+
+Hint Resolve inter_equal union_equal: core.
+
+Hint Resolve set_diff_elim1 set_diff_elim2 set_diff_intro set_diff_empty: core.
+Hint Resolve set_diff_IsOrd set_diff_nodup: core.
